Remove wcbv evaluation of axioms in PCUIC
In PCUIC we treated axioms as values, but we did not consistently treat
eg. fixpoints and cases stuck on axioms as values. This removes the
evaluation of axioms in PCUIC and gets rid of the axiom_free assumption
that was needed for erasure because of it.

pcuic/theories/PCUICCanonicity.v
@@ -802,7 +802,7 @@ Section WeakNormalization.
 
   Transparent construct_cofix_discr.
 
-  Lemma value_whnf t : closed t -> value Σ t -> wh_normal Σ [] t.
+  Lemma value_whnf t : closed t -> value t -> wh_normal Σ [] t.
   Proof.
     intros cl ev.
     induction ev in cl |- * using value_values_ind.
@@ -814,10 +814,6 @@ Section WeakNormalization.
       now rewrite nth_error_nil.
     - eapply (whnf_cofixapp _ _ [] _ _ []). 
     - unfold value_head in H. destruct t => //.
-      constructor; eapply whne_mkApps.
-      cbn in H; destruct lookup_env eqn:eq => //.
-      destruct g => //. destruct c => //. destruct cst_body => //.
-      eapply whne_const; eauto.
     - destruct f => //. cbn in H.
       destruct cunfold_fix as [[rarg body]|] eqn:unf => //.
       pose proof cl as cl'.
@@ -1014,41 +1010,92 @@ Section WeakNormalization.
     eapply PCUICConfluence.red_mkApps_tInd in r as [? [eq _]]; auto.
     solve_discr.
   Qed.
-
-  Lemma wh_neutral_empty_gen t Γ : axiom_free Σ -> wh_neutral Σ Γ t -> forall ty, Σ ;;; Γ |- t : ty -> Γ = [] -> False
-  with wh_normal_empty_gen t Γ i u args : axiom_free Σ -> wh_normal Σ Γ t -> Σ ;;; Γ |- t : mkApps (tInd i u) args -> 
-      Γ = [] -> construct_cofix_discr (head t).
+  
+  Fixpoint axiom_free_value Σ args t :=
+    match t with
+    | tApp hd arg => axiom_free_value Σ (axiom_free_value Σ [] arg :: args) hd
+    | tConst kn _ => match lookup_env Σ kn with
+                     | Some (ConstantDecl {| cst_body := Some _ |}) => true
+                     | _ => false
+                     end
+    | tCase _ _ discr _ => axiom_free_value Σ [] discr
+    | tProj _ t => axiom_free_value Σ [] t
+    | tFix defs i =>
+      match nth_error defs i with
+      | Some def => nth (rarg def) args true
+      | None => true
+      end
+    | _ => true
+    end.
+  
+  Lemma axiom_free_value_mkApps Σ' args hd args' :
+    axiom_free_value Σ' args (mkApps hd args') =
+    axiom_free_value Σ' (map (axiom_free_value Σ' []) args' ++ args) hd.
   Proof.
-    intros axfree ne ty typed.
-    2:intros axfree ne typed.
-    all:pose proof (subject_closed wfΣ typed) as cl;
-    destruct ne; intros eqΓ;  simpl in *; try discriminate.
-    - rewrite eqΓ in cl => //.
+    revert hd args.
+    induction args' using MCList.rev_ind; intros hd args; cbn; auto.
+    rewrite -mkApps_nested /=.
+    rewrite IHargs'.
+    now rewrite map_app /= -app_assoc.
+  Qed.
+  
+  Lemma wh_neutral_empty_gen Γ free t ty :
+    axiom_free_value Σ free t ->
+    wh_neutral Σ [] t ->
+    Σ ;;; Γ |- t : ty ->
+    Γ = [] ->
+    False.
+  Proof.
+    intros axfree ne typed.
+    induction ne in free, t, ty, axfree, ne, typed |- *; intros ->; simpl in *; try discriminate.
+    - apply inversion_Rel in typed as (?&?&?&?); auto.
+      rewrite nth_error_nil in e0; discriminate.
     - now eapply typing_var in typed.
     - now eapply typing_evar in typed.
-    - clear wh_neutral_empty_gen wh_normal_empty_gen. subst.
-      apply inversion_Const in typed as [decl' [wfd [declc [cu cum]]]]; eauto.
-      specialize (axfree  _ _ declc).
-      red in declc. rewrite declc in e. noconf e. congruence.
-    - simpl in cl; move/andP: cl => [clf cla].
-      eapply inversion_App in typed as [na [A [B [Hf _]]]]; eauto.
-    - specialize (wh_neutral_empty_gen _ _ axfree ne). subst.
-      simpl in cl. 
-      eapply inversion_mkApps in typed as (? & ? & ?); eauto.
+    - apply inversion_Const in typed as [decl' [wfd [declc [cu cum]]]]; eauto.
+      red in declc.
+      rewrite declc in e, axfree.
+      noconf e.
+      destruct decl; cbn in *.
+      rewrite e0 in axfree; congruence.
+    - eapply inversion_App in typed as [na [A [B [Hf _]]]]; eauto.
+    - eapply inversion_mkApps in typed as (? & ? & ?); eauto.
       eapply inversion_Fix in t as (? & ? & ? & ? & ? & ? & ?); auto.
       eapply typing_spine_strengthen in t0; eauto.
       eapply nth_error_all in a; eauto. simpl in a.
       rewrite /unfold_fix in e. rewrite e1 in e. noconf e.
       eapply (wf_fixpoint_spine wfΣ) in t0; eauto.
       rewrite e0 in t0. destruct t0 as [ind [u [indargs [tyarg ckind]]]].
-      clear wh_normal_empty_gen.
-      now specialize (wh_neutral_empty_gen _ tyarg eq_refl).
-    - move/andP: cl => [/andP[_ clc] _].
-      eapply inversion_Case in typed as (? & ? & ? & ? & ? & ? & ? & ? & ? & ? & ? & ? & ? & ? & ? & ? & ?); auto.
-      eapply wh_neutral_empty_gen; eauto.
-    - eapply inversion_Proj in typed as (? & ? & ? & ? & ? & ? & ? & ? & ?); auto.
-      eapply wh_neutral_empty_gen; eauto.
-    - eapply wh_neutral_empty_gen in w; eauto.
+      rewrite axiom_free_value_mkApps in axfree.
+      cbn in axfree.
+      rewrite e1 nth_nth_error nth_error_app1 in axfree.
+      1: { rewrite map_length.
+           apply nth_error_Some_length in e0; auto. }
+      rewrite nth_error_map e0 in axfree.
+      cbn in axfree.
+      eauto.
+    - eapply inversion_Case in typed as
+          (? & ? & ? & ? & ? & ? & ? & ? & ? & ? & ? & ? & ? & ? & ? & ? & ?); eauto.
+    - eapply inversion_Proj in typed as (? & ? & ? & ? & ? & ? & ? & ? & ?); eauto.
+  Qed.
+  
+  Lemma wh_neutral_empty t ty :
+    axiom_free_value Σ [] t ->
+    wh_neutral Σ [] t ->
+    Σ ;;; [] |- t : ty ->
+    False.
+  Proof. eauto using wh_neutral_empty_gen. Qed.
+  
+  Lemma wh_normal_ind_discr t i u args :
+    axiom_free_value Σ [] t ->
+    wh_normal Σ [] t ->
+    Σ ;;; [] |- t : mkApps (tInd i u) args -> 
+    construct_cofix_discr (head t).
+  Proof.
+    intros axfree ne typed.
+    pose proof (subject_closed wfΣ typed) as cl.
+    depelim ne; simpl in *.
+    - eauto using wh_neutral_empty.
     - eapply inversion_Sort in typed as (? & ? & ?); auto.
       eapply invert_cumul_sort_l in c as (? & ? & ?); auto.
       eapply red_mkApps_tInd in r as (? & eq & ?); eauto; eauto.
@@ -1068,20 +1115,8 @@ Section WeakNormalization.
     - now eapply inversion_Prim in typed.
   Qed.
 
-  Lemma wh_neutral_empty t ty : axiom_free Σ ->
-    Σ ;;; [] |- t : ty -> 
-    wh_neutral Σ [] t -> 
-    False.
-  Proof. intros; eapply wh_neutral_empty_gen; eauto. Qed.
-
-  Lemma wh_normal_ind_discr t i u args : axiom_free Σ -> 
-      Σ ;;; [] |- t : mkApps (tInd i u) args -> 
-      wh_normal Σ [] t -> 
-      construct_cofix_discr (head t).
-  Proof. intros. eapply wh_normal_empty_gen; eauto. Qed.
-
   Lemma whnf_ind_finite t ind u indargs : 
-    axiom_free Σ ->
+    axiom_free_value Σ [] t ->
     Σ ;;; [] |- t : mkApps (tInd ind u) indargs ->
     wh_normal Σ [] t ->
     check_recursivity_kind Σ (inductive_mind ind) Finite ->
@@ -1099,15 +1134,14 @@ Section WeakNormalization.
   Qed.
 
   Lemma fix_app_is_constructor {mfix idx args ty narg fn} : 
-    axiom_free Σ ->
     Σ;;; [] |- mkApps (tFix mfix idx) args : ty ->
     unfold_fix mfix idx = Some (narg, fn) ->
     match nth_error args narg return Type with
-    | Some a => wh_normal Σ [] a -> isConstruct_app a
+    | Some a => axiom_free_value Σ [] a -> wh_normal Σ [] a -> isConstruct_app a
     | None => ∑ na dom codom, Σ ;;; [] |- tProd na dom codom <= ty
     end.
   Proof.
-    intros axfree typed unf.
+    intros typed unf.
     eapply inversion_mkApps in typed as (? & ? & ?); eauto.
     eapply inversion_Fix in t as (? & ? & ? & ? & ? & ? & ?); auto.
     eapply typing_spine_strengthen in t0; eauto.
@@ -1117,9 +1151,31 @@ Section WeakNormalization.
     eapply (wf_fixpoint_spine wfΣ) in t0; eauto.
     rewrite /is_constructor. destruct (nth_error args (rarg x0)) eqn:hnth.
     destruct_sigma t0. destruct t0.
-    intros norm.
+    intros axfree norm.
     eapply whnf_ind_finite in t0; eauto.
     assumption.
+  Qed.
+  
+  Lemma value_axiom_free Σ' t :
+    value t ->
+    axiom_free_value Σ' [] t.
+  Proof.
+    intros val.
+    induction val using value_values_ind.
+    - destruct t; try discriminate; auto.
+      cbn.
+      destruct ?; auto.
+      destruct ?; auto.
+    - rewrite axiom_free_value_mkApps.
+      destruct t; auto.
+    - rewrite axiom_free_value_mkApps.
+      destruct f; try discriminate.
+      cbn.
+      unfold isStuckFix, cunfold_fix in H.
+      destruct nth_error; auto.
+      rewrite nth_overflow; auto.
+      rewrite app_nil_r map_length; auto.
+      toProp; auto.
   Qed.
 
   (** Evaluation on well-typed terms corresponds to reduction. 
@@ -1129,11 +1185,10 @@ Section WeakNormalization.
         have a constructor at their recursive argument as it is ensured by typing. *)
 
   Lemma wcbeval_red t ty u :
-    axiom_free Σ ->
     Σ ;;; [] |- t : ty ->
     eval Σ t u -> red Σ [] t u.
   Proof.
-  intros axfree Hc He.
+  intros Hc He.
   revert ty Hc.
   induction He; simpl; move=> ty Ht;
     try solve[econstructor; eauto].
@@ -1220,7 +1275,7 @@ Section WeakNormalization.
       eapply red_fix; eauto.
       assert (Σ ;;; [] |- mkApps (tFix mfix idx) (argsv ++ [av]) : B {0 := av}).
       { rewrite -mkApps_nested /=. eapply type_App'; eauto. }
-      epose proof (fix_app_is_constructor axfree X0 e); eauto.
+      epose proof (fix_app_is_constructor X0 e); eauto.
       rewrite /is_constructor.
       destruct nth_error eqn:hnth => //.
       assert (All (closedn 0) (argsv ++ [av])).
@@ -1228,7 +1283,7 @@ Section WeakNormalization.
         rewrite closedn_mkApps in X0.
         move/andP: X0 => [clfix clargs].
         now eapply forallb_All in clargs. }
-      assert (All (value Σ) (argsv ++ [av])).
+      assert (All value (argsv ++ [av])).
       { eapply All_app_inv; [|constructor; [|constructor]].
         eapply eval_to_value in He1.
         eapply value_mkApps_inv in He1 as [[[-> Hat]|[vh vargs]]|[hstuck vargs]] => //.
@@ -1236,6 +1291,7 @@ Section WeakNormalization.
       solve_all.
       eapply nth_error_all in X3; eauto. simpl in X3.
       destruct X3 as [cl val]. eapply X1, value_whnf; auto.
+      eapply value_axiom_free; auto.
       eapply nth_error_None in hnth; len in hnth; simpl in *. lia. }      
     redt _; eauto.
 
@@ -1273,14 +1329,15 @@ Section WeakNormalization.
   Qed.
 
   Lemma eval_ind_canonical t i u args : 
-    axiom_free Σ ->
     Σ ;;; [] |- t : mkApps (tInd i u) args -> 
     forall t', eval Σ t t' ->
     construct_cofix_discr (head t').
   Proof.
-    intros axfree Ht t' eval.
+    intros Ht t' eval.
     pose proof (subject_closed wfΣ Ht).
     eapply subject_reduction in Ht. 3:eapply wcbeval_red; eauto. 2:auto.
+    eapply eval_to_value in eval as axfree.
+    eapply value_axiom_free in axfree.
     eapply eval_whne in eval; auto.
     eapply wh_normal_ind_discr; eauto.
   Qed.
